added code definitions for several IO-set properties

Adaptive_State_Counting/FSM/FSM3.thy
@@ -272,6 +272,21 @@ lemma paths_of_length_path_set :
   "set (paths_of_length M q k) = { p . path M q p \<and> length p = k }"
 using paths_of_length_is_path[of _ M q k] paths_of_length_containment[of M q] by blast
 
+
+fun paths_up_to_length (* TODO *)
+
+
+
+
+
+
+
+
+
+
+
+
+
 fun language_state_for_input :: "'state FSM \<Rightarrow> 'state \<Rightarrow> Input list \<Rightarrow> (Input \<times> Output) list list" where
   "language_state_for_input M q xs = map p_io (filter (\<lambda> ts . xs = map t_input ts) (paths_of_length M q (length xs)))"
 
@@ -3323,14 +3338,67 @@ qed
 fun output_completion :: "(Input \<times> Output) list set \<Rightarrow> Output set \<Rightarrow> (Input \<times> Output) list set" where
   "output_completion P Out = P \<union> {io@[(fst xy, y)] | io xy y . y \<in> Out \<and> io@[xy] \<in> P \<and> io@[(fst xy, y)] \<notin> P}"
 
+
+
+
+
+
 fun output_complete_sequences :: "'a FSM \<Rightarrow> (Input \<times> Output) list set \<Rightarrow> bool" where
-  "output_complete_sequences M P = (\<forall> io xy y . io@[xy] \<in> P \<and> y \<in> set (outputs M) \<longrightarrow> io@[(fst xy, y)] \<in> P)"
+  "output_complete_sequences M P = (\<forall> io \<in> P . io = [] \<or> (\<forall> y \<in> set (outputs M) . (butlast io)@[(fst (last io), y)] \<in> P))"
+
+value "output_complete_sequences M_ex {}"  
+value "output_complete_sequences M_ex {[]}"
+value "output_complete_sequences M_ex {[],[(1,10)]}"
+value "output_complete_sequences M_ex {[],[(1,10)],[(1,20)]}"
+value "output_complete_sequences M_ex {[],[(1,10)],[(1,20)],[(1,30)]}"
+value "output_complete_sequences M_ex {[],[(1,10),(1,10)],[(1,20)],[(1,30)]}"
+value "output_complete_sequences M_ex {[],[(1,10),(1,10)],[(1,10),(1,20)],[(1,10),(1,30)]}"
+
+
 
 fun acyclic_sequences :: "'a FSM \<Rightarrow> (Input \<times> Output) list set \<Rightarrow> bool" where
   "acyclic_sequences M P = (\<forall> p . (path M (initial M) p \<and> p_io p \<in> P) \<longrightarrow> distinct (visited_states (initial M) p))"
 
+fun acyclic_sequences' :: "'a FSM \<Rightarrow> (Input \<times> Output) list set \<Rightarrow> bool" where
+  "acyclic_sequences' M P = (\<forall> io \<in> P . \<forall> p \<in> set (paths_of_length M (initial M) (length io)) . (p_io p = io) \<longrightarrow> distinct (visited_states (initial M) p))"
+
+lemma acyclic_sequences_alt_def[code] : "acyclic_sequences M P = acyclic_sequences' M P"
+  unfolding acyclic_sequences'.simps acyclic_sequences.simps
+  by (metis (no_types, lifting) length_map paths_of_length_containment paths_of_length_is_path(1))
+  
+value "acyclic_sequences M_ex {}"  
+value "acyclic_sequences M_ex {[]}"
+value "acyclic_sequences M_ex {[(1,30)]}"
+value "acyclic_sequences M_ex {[(1,30),(2,20)]}"
+
+
+
+
+
 fun single_input_sequences :: "'a FSM \<Rightarrow> (Input \<times> Output) list set \<Rightarrow> bool" where
   "single_input_sequences M P = (\<forall> xys1 xys2 xy1 xy2 . (xys1@[xy1] \<in> P \<and> xys2@[xy2] \<in> P \<and> io_target M xys1 (initial M) = io_target M xys2 (initial M)) \<longrightarrow> fst xy1 = fst xy2)"
+
+fun single_input_sequences' :: "'a FSM \<Rightarrow> (Input \<times> Output) list set \<Rightarrow> bool" where
+  "single_input_sequences' M P = (\<forall> io1 \<in> P . \<forall> io2 \<in> P . io1 = [] \<or> io2 = [] \<or> ((io_target M (butlast io1) (initial M) = io_target M (butlast io2) (initial M)) \<longrightarrow> fst (last io1) = fst (last io2)))"
+
+lemma single_input_sequences_alt_def[code] : "single_input_sequences M P = single_input_sequences' M P"
+  unfolding single_input_sequences.simps single_input_sequences'.simps
+  by (metis append_butlast_last_id append_is_Nil_conv butlast_snoc last_snoc not_Cons_self)
+
+value "single_input_sequences M_ex {}"
+value "single_input_sequences M_ex {[]}"
+value "single_input_sequences M_ex {[(1,30)]}"
+value "single_input_sequences M_ex {[(1,30)],[(2,30)]}"
+value "single_input_sequences M_ex {[(1,30)],[(1,20)]}"
+value "single_input_sequences M_ex {[(1,30)],[(1,30),(1,30)]}"
+value "single_input_sequences M_ex {[(1,30)],[(1,30),(2,30)]}"
+value "single_input_sequences M_ex {[(1,30)],[(1,30),(1,30)],[(1,30),(2,30)]}"
+
+
+
+
+
+
 
 fun output_complete_for_FSM_sequences :: "'a FSM \<Rightarrow> (Input \<times> Output) list set \<Rightarrow> bool" where
   "output_complete_for_FSM_sequences M P = (\<forall> io xy t . io@[xy] \<in> P \<and> t \<in> h M \<and> t_source t = io_target M io (initial M) \<and> t_input t = fst xy \<longrightarrow> io@[(fst xy, t_output t)] \<in> P)"
@@ -3377,19 +3445,91 @@ proof -
   qed 
 qed
 
+fun output_complete_for_FSM_sequences' :: "'a FSM \<Rightarrow> (Input \<times> Output) list set \<Rightarrow> bool" where
+  "output_complete_for_FSM_sequences' M P = (\<forall> io\<in>P . \<forall> t \<in> h M . io = [] \<or> (t_source t = io_target M (butlast io) (initial M) \<and> t_input t = fst (last io) \<longrightarrow> (butlast io)@[(fst (last io), t_output t)] \<in> P))"
+
+lemma output_complete_for_FSM_sequences_alt_def'[code] : "output_complete_for_FSM_sequences M P = output_complete_for_FSM_sequences' M P"
+  unfolding output_complete_for_FSM_sequences.simps output_complete_for_FSM_sequences'.simps
+  by (metis last_snoc snoc_eq_iff_butlast)
+  
+
+value "output_complete_for_FSM_sequences M_ex {}"
+value "output_complete_for_FSM_sequences M_ex {[]}"
+value "output_complete_for_FSM_sequences M_ex {[(1,20)]}"
+value "output_complete_for_FSM_sequences M_ex {[(1,10)],[(1,20)]}"
+value "output_complete_for_FSM_sequences M_ex {[(1,20)],[(1,30)]}"
+
   
 
 fun deadlock_states_sequences :: "'a FSM \<Rightarrow> 'a set \<Rightarrow> (Input \<times> Output) list set \<Rightarrow> bool" where
-  "deadlock_states_sequences M Q P = (\<forall> xys \<in> P . ((io_target M xys (initial M) \<in> Q 
-                                       \<and> \<not> (\<exists> xys' \<in> P . length xys < length xys' \<and> take (length xys) xys' = xys)))
-                                     \<or> (\<not> io_target M xys (initial M) \<in> Q 
+  "deadlock_states_sequences M Q P = (\<forall> xys \<in> P . 
+                                        ((io_target M xys (initial M) \<in> Q 
+                                          \<and> \<not> (\<exists> xys' \<in> P . length xys < length xys' \<and> take (length xys) xys' = xys)))
+                                      \<or> (\<not> io_target M xys (initial M) \<in> Q 
                                           \<and> (\<exists> xys' \<in> P . length xys < length xys' \<and> take (length xys) xys' = xys)))" 
+
+value "deadlock_states_sequences M_ex {} {}"
+value "deadlock_states_sequences M_ex {} {[]}"
+value "deadlock_states_sequences M_ex {2} {[]}" 
+value "deadlock_states_sequences M_ex {3} {[]}"
+value "deadlock_states_sequences M_ex {3} {[(1,20)]}"
+value "deadlock_states_sequences M_ex {2,3} {[(1,20)]}"
+value "deadlock_states_sequences M_ex {2,3} {[(1,30)]}"
+value "deadlock_states_sequences M_ex {2,4} {[],[(1,30)]}"
+value "deadlock_states_sequences M_ex {2,4} {[(1,20)],[(1,30)]}"
+value "deadlock_states_sequences M_ex {3,4} {[(1,20)],[(1,30)]}"
+
+
 
 fun reachable_states_sequences :: "'a FSM \<Rightarrow> 'a set \<Rightarrow> (Input \<times> Output) list set \<Rightarrow> bool" where
   "reachable_states_sequences M Q P = (\<forall> q \<in> Q . \<exists> xys \<in> P . io_target M xys (initial M) = q)"
 
+
+value "reachable_states_sequences M_ex {} {}"
+value "reachable_states_sequences M_ex {} {[]}"
+value "reachable_states_sequences M_ex {2} {}"
+value "reachable_states_sequences M_ex {2} {[]}"
+value "reachable_states_sequences M_ex {3,4} {[(1,20)],[(1,30),(2,20)]}"
+value "reachable_states_sequences M_ex {3,4} {[(1,20)],[(1,30)]}"
+value "reachable_states_sequences M_ex {3,4,5} {[(1,20)],[(1,30)]}"
+
+
 fun prefix_closed_sequences :: "(Input \<times> Output) list set \<Rightarrow> bool" where
   "prefix_closed_sequences P = (\<forall> xys1 xys2 . xys1@xys2 \<in> P \<longrightarrow> xys1 \<in> P)"
+
+fun prefix_closed_sequences' :: "(Input \<times> Output) list set \<Rightarrow> bool" where
+  "prefix_closed_sequences' P = (\<forall> io \<in> P . io = [] \<or> (butlast io) \<in> P)"
+
+lemma prefix_closed_sequences_alt_def[code] : "prefix_closed_sequences P = prefix_closed_sequences' P"
+proof 
+  show "prefix_closed_sequences P \<Longrightarrow> prefix_closed_sequences' P"
+    unfolding prefix_closed_sequences.simps prefix_closed_sequences'.simps
+    by (metis append_butlast_last_id) 
+
+  have "\<And>xys1 xys2. \<forall>io\<in>P. io = [] \<or> butlast io \<in> P \<Longrightarrow> xys1 @ xys2 \<in> P \<Longrightarrow> xys1 \<in> P"
+  proof -
+    fix xys1 xys2 assume "\<forall>io\<in>P. io = [] \<or> butlast io \<in> P" and "xys1 @ xys2 \<in> P"
+    then show "xys1 \<in> P"
+    proof (induction xys2 rule: rev_induct)
+      case Nil
+      then show ?case by auto
+    next
+      case (snoc a xys2)
+      then show ?case
+        by (metis append.assoc snoc_eq_iff_butlast) 
+    qed
+  qed
+
+  then show "prefix_closed_sequences' P \<Longrightarrow> prefix_closed_sequences P"
+    unfolding prefix_closed_sequences.simps prefix_closed_sequences'.simps by blast 
+qed
+
+value "prefix_closed_sequences {}"
+value "prefix_closed_sequences {[]}"
+value "prefix_closed_sequences {[(1,20)]}"
+value "prefix_closed_sequences {[],[(1,20)]}"
+
+
 
 lemma is_preamble_set_alt_def :
   "is_preamble_set M q P = (
@@ -3408,8 +3548,17 @@ lemma is_preamble_set_alt_def :
             reachable_states_sequences.simps
             prefix_closed_sequences.simps 
   by blast
-  
 
+
+fun list_max :: "nat list \<Rightarrow> nat" where
+  "list_max [] = 0" |
+  "list_max xs = Max (set xs)"
+
+lemma list_max_is_max : "q \<in> set xs \<Longrightarrow> q \<le> list_max xs"
+  by (metis List.finite_set Max_ge length_greater_0_conv length_pos_if_in_set list_max.elims) 
+
+
+lemma language_subset_code[code] : "((set P) \<subseteq> L M) = ((set P) \<subseteq> (set (map p_io (paths_of_length M (initial M) (list_max (map length P))))))"
             
 
 (* test cases *)
